coq/DNNRC/Calculus/DNNRCEq.v
@@ -28,16 +28,18 @@ Section DNNRCEq.
   Require Import Utils BasicRuntime.
   Require Import DData DDataNorm DNNRC.
 
-  Context {A:Type}.
+  Context {fruntime:foreign_runtime}.
+  Context {A plug_type:Set}.
   Context {eqdec:EqDec A eq}.
-  Context `{plug:AlgPlug}.
+  Context {plug:AlgPlug plug_type}.
 
-  (** Equivalence between expressions in the Named Nested Relational Calculus *)
+  (** Equivalence between expressions in the 
+      Distributed Nested Relational Calculus *)
 
-  Definition dnnrc_eq (e1 e2:dnrc) : Prop :=
-    forall (denv:dbindings),
+  Definition dnnrc_eq (e1 e2:dnrc A plug_type) : Prop :=
+    forall (h:brand_relation_t) (denv:dbindings),
       Forall (ddata_normalized h) (map snd denv) ->
-      @dnrc_eval _ h A T plug denv e1 = @dnrc_eval _ h A T plug denv e2.
+      dnrc_eval h denv e1 = dnrc_eval h denv e2.
 
   Global Instance dnnrc_equiv : Equivalence dnnrc_eq.
   Proof.
@@ -45,10 +47,10 @@ Section DNNRCEq.
     - unfold Reflexive, dnnrc_eq.
       intros; reflexivity.
     - unfold Symmetric, dnnrc_eq.
-      intros; rewrite (H denv) by trivial; reflexivity.
+      intros; rewrite (H _ denv) by trivial; reflexivity.
     - unfold Transitive, dnnrc_eq.
-      intros; rewrite (H denv) by trivial;
-      rewrite (H0 denv) by trivial; reflexivity.
+      intros; rewrite (H _ denv) by trivial;
+      rewrite (H0 _ denv) by trivial; reflexivity.
   Qed.
 
   (* all the dnnrc constructors are proper wrt. equivalence *)
@@ -76,12 +78,12 @@ Section DNNRCEq.
     intros; simpl. subst.
     rewrite H1 by trivial.
     rewrite H2 by trivial.
-    case_eq (@dnrc_eval _ _ _ _ plug denv y1);
-      case_eq (@dnrc_eval _ _ _ _ plug denv y2); intros; simpl; trivial.
+    case_eq (dnrc_eval h denv y1);
+      case_eq (dnrc_eval h denv y2); intros; simpl; trivial.
     destruct d0; destruct d; try reflexivity; simpl.
     rewrite H0; [reflexivity| | ].
-    apply (@dnrc_eval_normalized_local _ _ _ _ plug denv y1); try assumption.
-    apply (@dnrc_eval_normalized_local _ _ _ _ plug denv y1); try assumption.
+    apply (dnrc_eval_normalized_local h denv y1); try assumption.
+    apply (dnrc_eval_normalized_local h denv y1); try assumption.
   Qed.
 
   (* DNRCUnnop *)
@@ -91,10 +93,10 @@ Section DNNRCEq.
     unfold Proper, respectful, dnnrc_eq.
     intros; simpl. subst.
     rewrite H1 by trivial.
-    case_eq (dnrc_eval denv y1); simpl; trivial; intros.
+    case_eq (dnrc_eval h denv y1); simpl; trivial; intros.
     destruct d; try reflexivity; simpl.
     rewrite H0; [reflexivity| ].
-    apply (@dnrc_eval_normalized_local _ _ _ _ plug denv y1); try assumption.
+    apply (dnrc_eval_normalized_local h denv y1); try assumption.
   Qed.
     
   (* DNRCLet *)
@@ -103,11 +105,11 @@ Section DNNRCEq.
   Proof.
     unfold Proper, respectful, dnnrc_eq.
     intros; simpl. rewrite H0; clear H0; rewrite H1 by trivial; clear H1.
-    case_eq (dnrc_eval denv y1); simpl; trivial; intros.
+    case_eq (dnrc_eval h denv y1); simpl; trivial; intros.
     rewrite H2; eauto.
     constructor; eauto.
     simpl.
-    apply (@dnrc_eval_normalized _ _ _ _ plug denv y1 d); try assumption.
+    eapply dnrc_eval_normalized; eauto.
   Qed.
 
   (* DNRCFor *)
@@ -118,7 +120,7 @@ Section DNNRCEq.
   Proof.
     unfold Proper, respectful, dnnrc_eq.
     intros; simpl. rewrite H1 by trivial; clear H1. subst.
-    case_eq (dnrc_eval denv y1); simpl; trivial; intros.
+    case_eq (dnrc_eval h denv y1); simpl; trivial; intros.
     destruct d; try reflexivity; simpl.
     destruct d; try reflexivity; simpl.
     f_equal.
@@ -126,12 +128,12 @@ Section DNNRCEq.
     rewrite H2; simpl; eauto.
     constructor; [|assumption].
     assert (ddata_normalized h (Dlocal (dcoll l))).
-    apply (@dnrc_eval_normalized _ _ _ _ plug denv y1); assumption.
-    inversion H1; subst; clear H1.
-    constructor.
-    inversion H5; subst; clear H5.
-    rewrite Forall_forall in H4.
-    auto.
+    - eapply dnrc_eval_normalized; eauto.
+    - inversion H1; subst; clear H1.
+      constructor.
+      inversion H5; subst; clear H5.
+      rewrite Forall_forall in H4.
+      auto.
   Qed.
 
   (* DNRCIf *)
@@ -140,7 +142,7 @@ Section DNNRCEq.
   Proof.
     unfold Proper, respectful, dnnrc_eq.
     intros; simpl. subst. rewrite H0 by trivial; clear H0.
-    case_eq (dnrc_eval denv y0); simpl; trivial; intros.
+    case_eq (dnrc_eval h denv y0); simpl; trivial; intros.
     destruct d; try reflexivity; simpl.
     destruct d; try reflexivity; simpl.
     destruct b; eauto.
@@ -157,7 +159,7 @@ Section DNNRCEq.
       rewrite Forall_forall; intros.
       inversion H; subst.
       unfold olift, checkLocal in eqq1.
-      case_eq (dnrc_eval denv y0); intros; rewrite H1 in eqq1; try congruence;
+      case_eq (dnrc_eval h denv y0); intros; rewrite H1 in eqq1; try congruence;
       destruct d0; try congruence; inversion eqq1; subst.
       assert (ddata_normalized h (Dlocal (dleft d))).
       apply (@dnrc_eval_normalized _ _ _ _ plug denv y0); assumption.
@@ -169,7 +171,7 @@ Section DNNRCEq.
       rewrite Forall_forall; intros.
       inversion H; subst.
       unfold olift, checkLocal in eqq1.
-      case_eq (dnrc_eval denv y0); intros; rewrite H1 in eqq1; try congruence;
+      case_eq (dnrc_eval h denv y0); intros; rewrite H1 in eqq1; try congruence;
       destruct d0; try congruence; inversion eqq1; subst.
       assert (ddata_normalized h (Dlocal (dright d))).
       apply (@dnrc_eval_normalized _ _ _ _ plug denv y0); assumption.
